Recall,

`S = { 3n | n ∊ ℕ }`.

Let `R = { 3n+1 | n ∊ ℕ }` and put `T = S U R`.

Then,

1. `0 ∊ T` since `0 ∊ S` and `S` is a subset of `T`.

2. Assume `n ∊ T`. Either `n ∊ S` or `n ∊ R`. Case 1, `n ∊ S` implies that
`n+3 ∊ S` due to the way `S` was defined. And so `n+3 ∊ T` since `S` is a
subset of `T`. Case 2, `n ∊ R` implies that `n=3k+1` for some `k ∊ ℕ`. Now,
`n+3=(3k+1)+3=(3k+3)+1=3(k+1)+1 ∊ R`. And so `n+3 ∊ T` since `R` is a subset
of `T`. Therefore, whenever `n ∊ T` then `n+3 ∊ T`.

3. `T ≠ S` since 1 is in `T` but 1 is not in `S`.
